theories/soundness.v
@@ -3,13 +3,13 @@ Require Import fp_red logrel typing.
 From Hammer Require Import Tactics.
 
 Theorem fundamental_theorem :
-  (forall n (Γ : fin n -> PTm n), ⊢ Γ -> ⊨ Γ) /\
-  (forall n Γ (a A : PTm n), Γ ⊢ a ∈ A -> Γ ⊨ a ∈ A)  /\
-  (forall n Γ (a b A : PTm n), Γ ⊢ a ≡ b ∈ A -> Γ ⊨ a ≡ b ∈ A) /\
-  (forall n Γ (a b : PTm n), Γ ⊢ a ≲ b -> Γ ⊨ a ≲ b).
+  (forall Γ, ⊢ Γ -> ⊨ Γ) /\
+  (forall Γ a A, Γ ⊢ a ∈ A -> Γ ⊨ a ∈ A)  /\
+  (forall Γ a b A, Γ ⊢ a ≡ b ∈ A -> Γ ⊨ a ≡ b ∈ A) /\
+  (forall Γ a b, Γ ⊢ a ≲ b -> Γ ⊨ a ≲ b).
   apply wt_mutual; eauto with sem; [hauto l:on use:SE_Pair].
   Unshelve. all : exact 0.
 Qed.
 
-Lemma synsub_to_usub : forall n Γ (a b : PTm n), Γ ⊢ a ≲ b -> SN a /\ SN b /\ Sub.R a b.
+Lemma synsub_to_usub : forall Γ (a b : PTm), Γ ⊢ a ≲ b -> SN a /\ SN b /\ Sub.R a b.
 Proof. hauto lq:on rew:off use:fundamental_theorem, SemLEq_SN_Sub. Qed.
